chore

Auto/Embedding/LCtx.lean
@@ -40,70 +40,117 @@ theorem pushLCtxDep.absorb {rty : Nat → α} {lctxty : α → Sort u}
     (@pushLCtxDep _ rty lctxty lctx _ x) (@pushLCtxDep _ (lctxty ∘ rty) id lctx _ x) :=
   PSigmaEq.of_heq _ (HEq.funext _ _ (pushLCtxDep.absorbAux _ _)) (pushLCtx.commFn _ _ _)
 
-def pushLCtxAt (lctx : Nat → α) (x : α) : (pos : Nat) → Nat → α
+def pushLCtxAt (lctx : Nat → α) (x : α) (pos n : Nat) : α :=
+  match n.ble pos with
+  | true => 
+    match n.beq pos with
+    | true => x
+    | false => lctx n
+  | false => lctx (.pred n)
+
+def pushLCtxAtRec (lctx : Nat → α) (x : α) : (pos : Nat) → Nat → α
 | 0 => pushLCtx lctx x
 | pos' + 1 => fun n =>
   match n with
   | 0 => lctx 0
-  | n' + 1 => pushLCtxAt (fun n => lctx (Nat.succ n)) x pos' n'
+  | n' + 1 => pushLCtxAtRec (fun n => lctx (Nat.succ n)) x pos' n'
 
-def pushLCtxAt.comm (f : α → β) (lctx : Nat → α) (x : α) :
-  (pos : Nat) → (n : Nat) → f (pushLCtxAt lctx x pos n) = pushLCtxAt (f ∘ lctx) (f x) pos n
+theorem pushLCtxAt.equiv (lctx : Nat → α) (x : α) (pos n : Nat) :
+  pushLCtxAtRec lctx x pos n = pushLCtxAt lctx x pos n := by
+  revert lctx n; induction pos <;> intro lctx n
+  case zero =>
+    cases n <;> rfl
+  case succ pos' IH =>
+    cases n
+    case zero => rfl
+    case succ n' =>
+      let IH' := IH (fun n => lctx (.succ n)) n'
+      dsimp [pushLCtxAtRec, pushLCtxAt, Nat.ble, Nat.beq]
+      dsimp [pushLCtxAtRec, pushLCtxAt, Nat.ble, Nat.beq] at IH'
+      cases n'
+      case zero =>
+        rw [Nat.ble_eq_true_of_le (Nat.zero_le _)]; dsimp
+        rw [Nat.ble_eq_true_of_le (Nat.zero_le _)] at IH'; dsimp at IH'
+        exact IH'
+      case succ n' =>
+        exact IH'
+
+def pushLCtxAtRec.comm (f : α → β) (lctx : Nat → α) (x : α) :
+  (pos : Nat) → (n : Nat) → f (pushLCtxAtRec lctx x pos n) = pushLCtxAtRec (f ∘ lctx) (f x) pos n
 | 0 => fun n => by
-  dsimp [pushLCtxAt]; apply pushLCtx.comm
+  dsimp [pushLCtxAtRec]; apply pushLCtx.comm
 | pos' + 1 => fun n =>
   match n with
   | 0 => rfl
-  | n' + 1 => pushLCtxAt.comm f (fun n => lctx (Nat.succ n)) x pos' n'
+  | n' + 1 => pushLCtxAtRec.comm f (fun n => lctx (Nat.succ n)) x pos' n'
 
-theorem pushLCtxAt.commFn (lctx : Nat → α) (f : α → β) (x : α) (pos : Nat) :
-  (fun n => f (pushLCtxAt lctx x pos n)) = (fun n => pushLCtxAt (fun n => f (lctx n)) (f x) pos n) :=
-  funext (pushLCtxAt.comm f lctx x pos)
+theorem pushLCtxAtRec.commFn (lctx : Nat → α) (f : α → β) (x : α) (pos : Nat) :
+  (fun n => f (pushLCtxAtRec lctx x pos n)) = (fun n => pushLCtxAtRec (fun n => f (lctx n)) (f x) pos n) :=
+  funext (pushLCtxAtRec.comm f lctx x pos)
 
 -- Surprisingly, this is definitionally equal
-def pushLCtx_pushLCtxAt (lctx : Nat → α) (x y : α) (pos : Nat) :
-  pushLCtx (pushLCtxAt lctx x pos) y = pushLCtxAt (pushLCtx lctx y) x (Nat.succ pos)
+def pushLCtx_pushLCtxAtRec (lctx : Nat → α) (x y : α) (pos : Nat) :
+  pushLCtx (pushLCtxAtRec lctx x pos) y = pushLCtxAtRec (pushLCtx lctx y) x (Nat.succ pos)
   := rfl
 
 def pushLCtxAtDep {rty : Nat → α} {lctxty : α → Sort u}
-  (lctx : ∀ n, lctxty (rty n)) {xty : α} (x : lctxty xty) : (pos : Nat) → (n : Nat) → lctxty (pushLCtxAt rty xty pos n)
+  (lctx : ∀ n, lctxty (rty n)) {xty : α} (x : lctxty xty) (pos n : Nat) : lctxty (pushLCtxAt rty xty pos n) := by
+  dsimp [pushLCtxAt]
+  match n.ble pos with
+  | true =>
+    match n.beq pos with
+    | true => exact x
+    | false => exact (lctx n)
+  | false => exact (lctx (.pred n))
+
+def pushLCtxAtDepRec {rty : Nat → α} {lctxty : α → Sort u}
+  (lctx : ∀ n, lctxty (rty n)) {xty : α} (x : lctxty xty) : (pos : Nat) → (n : Nat) → lctxty (pushLCtxAtRec rty xty pos n)
 | 0 => pushLCtxDep lctx x
 | pos' + 1 => fun n =>
   match n with
   | 0 => lctx 0
-  | n' + 1 => pushLCtxAtDep (fun n => lctx (Nat.succ n)) x pos' n'
+  | n' + 1 => pushLCtxAtDepRec (fun n => lctx (Nat.succ n)) x pos' n'
 
-def pushLCtxAtDep.comm {α : Sort w} {β : α → Sort x} {rty : Nat → α} {lctxty : α → Sort u}
+def pushLCtxAtDep.equiv {rty : Nat → α} {lctxty : α → Sort u}
+  (lctx : ∀ n, lctxty (rty n)) {xty : α} (x : lctxty xty) (pos n : Nat) :
+  HEq (pushLCtxAtDepRec lctx x n) (pushLCtxAtDep lctx x n) := by
+  dsimp [pushLCtxAtDep]; revert lctx n; induction pos <;> intro lctx n
+  case zero =>
+    sorry
+  case succ =>
+    sorry  
+
+def pushLCtxAtDepRec.comm {α : Sort w} {β : α → Sort x} {rty : Nat → α} {lctxty : α → Sort u}
   (f : ∀ (x : α), lctxty x → β x) (lctx : ∀ n, lctxty (rty n))
   {xty : α} (x : lctxty xty) : (pos : Nat) → (n : Nat) →
-    f _ (pushLCtxAtDep lctx x pos n) = pushLCtxAtDep (lctxty:=β) (fun n => f _ (lctx n)) (f xty x) pos n
+    f _ (pushLCtxAtDepRec lctx x pos n) = pushLCtxAtDepRec (lctxty:=β) (fun n => f _ (lctx n)) (f xty x) pos n
 | 0 => fun _ => pushLCtxDep.comm _ _ _ _
 | pos' + 1 => fun n =>
   match n with
   | 0 => rfl
-  | n' + 1 => pushLCtxAtDep.comm f (fun n => lctx (Nat.succ n)) x pos' n'
+  | n' + 1 => pushLCtxAtDepRec.comm f (fun n => lctx (Nat.succ n)) x pos' n'
 
-def pushLCtxAtDep.absorbAux {rty : Nat → α} {lctxty : α → Sort u}
+def pushLCtxAtDepRec.absorbAux {rty : Nat → α} {lctxty : α → Sort u}
   (lctx : ∀ n, lctxty (rty n)) {xty : α} (x : lctxty xty) :
   (pos : Nat) → (n : Nat) → HEq
-    (@pushLCtxAtDep _ rty lctxty lctx _ x pos n)
-    (@pushLCtxAtDep _ (lctxty ∘ rty) id lctx _ x pos n)
+    (@pushLCtxAtDepRec _ rty lctxty lctx _ x pos n)
+    (@pushLCtxAtDepRec _ (lctxty ∘ rty) id lctx _ x pos n)
 | 0 => fun _ => pushLCtxDep.absorbAux _ _ _
 | pos' + 1 => fun n =>
   match n with
   | 0 => HEq.refl _
-  | n' + 1 => pushLCtxAtDep.absorbAux (fun n => lctx (.succ n)) x pos' n'
+  | n' + 1 => pushLCtxAtDepRec.absorbAux (fun n => lctx (.succ n)) x pos' n'
 
-theorem pushLCtxAtDep.absorb {rty : Nat → α} {lctxty : α → Sort u}
+theorem pushLCtxAtDepRec.absorb {rty : Nat → α} {lctxty : α → Sort u}
   (lctx : ∀ n, lctxty (rty n)) {xty : α} (x : lctxty xty) (pos : Nat) :
   PSigmaEq (fun (α : Nat → Sort u) => (∀ (n : Nat), α n))
-    (@pushLCtxAtDep _ rty lctxty lctx _ x pos) (@pushLCtxAtDep _ (lctxty ∘ rty) id lctx _ x pos) :=
-  PSigmaEq.of_heq _ (HEq.funext _ _ (pushLCtxAtDep.absorbAux _ _ _)) (pushLCtxAt.commFn _ _ _ _)
+    (@pushLCtxAtDepRec _ rty lctxty lctx _ x pos) (@pushLCtxAtDepRec _ (lctxty ∘ rty) id lctx _ x pos) :=
+  PSigmaEq.of_heq _ (HEq.funext _ _ (pushLCtxAtDepRec.absorbAux _ _ _)) (pushLCtxAtRec.commFn _ _ _ _)
 
 -- Surprisingly, this is definitionally equal
-def pushLCtxDep_pushLCtxAtDep {rty : Nat → α} {lctxty : α → Sort u}
+def pushLCtxDep_pushLCtxAtDepRec {rty : Nat → α} {lctxty : α → Sort u}
   (lctx : ∀ n, lctxty (rty n)) {xty : α} (x : lctxty xty) {yty : α} (y : lctxty yty) (pos : Nat) :
-  pushLCtxDep (pushLCtxAtDep lctx x pos) y = pushLCtxAtDep (pushLCtxDep lctx y) x (Nat.succ pos) := rfl
+  pushLCtxDep (pushLCtxAtDepRec lctx x pos) y = pushLCtxAtDepRec (pushLCtxDep lctx y) x (Nat.succ pos) := rfl
 
 def popLCtx (lctx : Nat → α) := fun n => lctx (n + 1)
 
@@ -131,78 +178,100 @@ theorem popLCtxDep.absorb {rty : Nat → α} {lctxty : α → Sort u} (lctx : �
     (@popLCtxDep _ rty lctxty lctx) (@popLCtxDep _ (lctxty ∘ rty) id lctx) :=
   PSigmaEq.of_heq _ (HEq.funext _ _ (popLCtxDep.absorbAux _)) (popLCtx.commFn _ _)
 
-def popLCtxAt (lctx : Nat → α) (pos : Nat) := 
+def popLCtxAt (lctx : Nat → α) (pos n : Nat) :=
+  match pos.ble n with
+  | true => lctx (.succ n)
+  | false => lctx n
+
+def popLCtxAtRec (lctx : Nat → α) (pos : Nat) := 
   match pos with
   | 0 => popLCtx lctx
   | pos' + 1 => fun n =>
     match n with
     | 0 => lctx 0
-    | n' + 1 => popLCtxAt (fun n => lctx (Nat.succ n)) pos' n'
+    | n' + 1 => popLCtxAtRec (fun n => lctx (Nat.succ n)) pos' n'
 
-def popLCtxAt.comm (lctx : Nat → α) (f : α → β) (pos : Nat) :
-  (n : Nat) → f (popLCtxAt lctx pos n) = popLCtxAt (f ∘ lctx) pos n :=
+theorem popLCtxAt.equiv (lctx : Nat → α) (pos n : Nat) :
+  popLCtxAtRec lctx pos n = popLCtxAt lctx pos n := by
+  revert lctx n; induction pos <;> intro lctx n
+  case zero =>
+    cases n <;> rfl
+  case succ pos' IH =>
+    cases n
+    case zero => rfl
+    case succ n' => exact (IH (fun n => lctx (.succ n)) n')
+
+def popLCtxAtRec.comm (lctx : Nat → α) (f : α → β) (pos : Nat) :
+  (n : Nat) → f (popLCtxAtRec lctx pos n) = popLCtxAtRec (f ∘ lctx) pos n :=
   match pos with
   | 0 => fun _ => rfl
   | pos' + 1 => fun n =>
     match n with
     | 0 => rfl
-    | n' + 1 => popLCtxAt.comm (fun n => lctx (.succ n)) f pos' n'
+    | n' + 1 => popLCtxAtRec.comm (fun n => lctx (.succ n)) f pos' n'
 
-def popLCtxAt.commFn (lctx : Nat → α) (f : α → β) (pos : Nat) :
-  (fun n => f (popLCtxAt lctx pos n)) = (fun n => popLCtxAt (f ∘ lctx) pos n) :=
-  funext (popLCtxAt.comm lctx f pos)
+def popLCtxAtRec.commFn (lctx : Nat → α) (f : α → β) (pos : Nat) :
+  (fun n => f (popLCtxAtRec lctx pos n)) = (fun n => popLCtxAtRec (f ∘ lctx) pos n) :=
+  funext (popLCtxAtRec.comm lctx f pos)
 
 def popLCtxAtDep {rty : Nat → α} {lctxty : α → Sort u}
-  (lctx : ∀ n, lctxty (rty n)) : (pos : Nat) → (n : Nat) → lctxty (popLCtxAt rty pos n)
+  (lctx : ∀ n, lctxty (rty n)) (pos : Nat) (n : Nat) : lctxty (popLCtxAt rty pos n) := by
+  dsimp [popLCtxAt]
+  match pos.ble n with
+  | true => exact lctx (.succ n)
+  | false => exact lctx n
+
+def popLCtxAtDepRec {rty : Nat → α} {lctxty : α → Sort u}
+  (lctx : ∀ n, lctxty (rty n)) : (pos : Nat) → (n : Nat) → lctxty (popLCtxAtRec rty pos n)
 | 0 => popLCtxDep lctx
 | pos' + 1 => fun n =>
   match n with
   | 0 => lctx 0
-  | n' + 1 => popLCtxAtDep (fun n => lctx (Nat.succ n)) pos' n'
+  | n' + 1 => popLCtxAtDepRec (fun n => lctx (Nat.succ n)) pos' n'
 
-def popLCtxAtDep.absorbAux {rty : Nat → α} {lctxty : α → Sort u}
+def popLCtxAtDepRec.absorbAux {rty : Nat → α} {lctxty : α → Sort u}
   (lctx : ∀ n, lctxty (rty n)) : (pos : Nat) → (n : Nat) → HEq
-    (@popLCtxAtDep _ rty lctxty lctx pos n)
-    (@popLCtxAtDep _ (lctxty ∘ rty) id lctx pos n)
+    (@popLCtxAtDepRec _ rty lctxty lctx pos n)
+    (@popLCtxAtDepRec _ (lctxty ∘ rty) id lctx pos n)
 | 0 => fun _ => HEq.refl _
 | pos' + 1 => fun n =>
   match n with
   | 0 => HEq.refl _
-  | n' + 1 => popLCtxAtDep.absorbAux (fun n => lctx (.succ n)) pos' n'
+  | n' + 1 => popLCtxAtDepRec.absorbAux (fun n => lctx (.succ n)) pos' n'
 
-def popLCtxAtDep.absorbAux' {rty : Nat → α} {lctxty : α → Sort u}
+def popLCtxAtDepRec.absorbAux' {rty : Nat → α} {lctxty : α → Sort u}
   (lctx : ∀ n, lctxty (rty n)) (pos : Nat) (n : Nat) : HEq
-    (@popLCtxAtDep _ rty lctxty lctx pos n)
-    (@popLCtxAtDep _ id (lctxty ∘ rty) lctx pos n) :=
+    (@popLCtxAtDepRec _ rty lctxty lctx pos n)
+    (@popLCtxAtDepRec _ id (lctxty ∘ rty) lctx pos n) :=
   HEq.trans
-    (b := @popLCtxAtDep _ (lctxty ∘ rty) id lctx pos n)
-    (popLCtxAtDep.absorbAux lctx pos n)
-    (HEq.symm (@popLCtxAtDep.absorbAux _ id (lctxty ∘ rty) lctx pos n))
+    (b := @popLCtxAtDepRec _ (lctxty ∘ rty) id lctx pos n)
+    (popLCtxAtDepRec.absorbAux lctx pos n)
+    (HEq.symm (@popLCtxAtDepRec.absorbAux _ id (lctxty ∘ rty) lctx pos n))
 
-def popLCtxAtDep.absorb {rty : Nat → α} {lctxty : α → Sort u} (lctx : ∀ n, lctxty (rty n)) (pos : Nat):
+def popLCtxAtDepRec.absorb {rty : Nat → α} {lctxty : α → Sort u} (lctx : ∀ n, lctxty (rty n)) (pos : Nat):
   PSigmaEq (fun (α : Nat → Sort u) => (∀ (n : Nat), α n))
-    (@popLCtxAtDep _ rty lctxty lctx pos) (@popLCtxAtDep _ (lctxty ∘ rty) id lctx pos) :=
-  PSigmaEq.of_heq _ (HEq.funext _ _ (popLCtxAtDep.absorbAux _ _)) (popLCtxAt.commFn _ _ _)
+    (@popLCtxAtDepRec _ rty lctxty lctx pos) (@popLCtxAtDepRec _ (lctxty ∘ rty) id lctx pos) :=
+  PSigmaEq.of_heq _ (HEq.funext _ _ (popLCtxAtDepRec.absorbAux _ _)) (popLCtxAtRec.commFn _ _ _)
 
-def popLCtxAtDep.comm {α : Sort w} {β : α → Sort x} {rty : Nat → α} {lctxty : α → Sort u}
+def popLCtxAtDepRec.comm {α : Sort w} {β : α → Sort x} {rty : Nat → α} {lctxty : α → Sort u}
   (f : ∀ (x : α), lctxty x → β x) (lctx : ∀ n, lctxty (rty n)) :
-  (pos : Nat) → (n : Nat) → f _ (popLCtxAtDep lctx pos n) = popLCtxAtDep (lctxty:=β) (fun n => f _ (lctx n)) pos n
+  (pos : Nat) → (n : Nat) → f _ (popLCtxAtDepRec lctx pos n) = popLCtxAtDepRec (lctxty:=β) (fun n => f _ (lctx n)) pos n
 | 0 => fun _ => rfl
 | pos' + 1 => fun n =>
   match n with
   | 0 => rfl
-  | n' + 1 => popLCtxAtDep.comm f (fun n => lctx (Nat.succ n)) pos' n'
+  | n' + 1 => popLCtxAtDepRec.comm f (fun n => lctx (Nat.succ n)) pos' n'
 
-def popLCtxAt.commDep
+def popLCtxAtRec.commDep
   {β : α → Sort u} (lctx : Nat → α) (f : ∀ (x : α), β x) :
-  (pos n : Nat) → f (popLCtxAt lctx pos n) = popLCtxAtDep (fun n => f (lctx n)) pos n
+  (pos n : Nat) → f (popLCtxAtRec lctx pos n) = popLCtxAtDepRec (fun n => f (lctx n)) pos n
 | 0 => fun _ => rfl
 | pos' + 1 => fun n =>
   match n with
   | 0 => rfl
-  | n' + 1 => popLCtxAt.commDep (fun n => lctx (.succ n)) f pos' n'
+  | n' + 1 => popLCtxAtRec.commDep (fun n => lctx (.succ n)) f pos' n'
  
--- #reduce fun lctx => popLCtxAt lctx 3 4
+-- #reduce fun lctx => popLCtxAtRec lctx 3 4
 
 def popLCtxs (lctx : Nat → α) : (i : Nat) → Nat → α
 | 0 => lctx
@@ -215,34 +284,34 @@ def popLCtxs (lctx : Nat → α) : (i : Nat) → Nat → α
 -- #reduce fun lctx x => popLCtx (pushLCtx lctx x)
 --   popLCtxs lctx 0 = lctx
 -- #reduce fun lctx => popLCtxs lctx 0
--- #reduce fun lctx x => pushLCtxAt lctx x (pos:=2) 4
+-- #reduce fun lctx x => pushLCtxAtRec lctx x (pos:=2) 4
 -- #reduce (fun lctx x y t => (Eq.refl _ :
---   pushLCtx (pushLCtxAt lctx x t) y = pushLCtxAt (pushLCtx lctx y) x (t + 1)))
+--   pushLCtx (pushLCtxAtRec lctx x t) y = pushLCtxAtRec (pushLCtx lctx y) x (t + 1)))
 
 def push_pop_eq (lctx : Nat → α) :
   pushLCtx (popLCtx lctx) (lctx 0) = lctx := by
   apply funext
   intro n; cases n <;> rfl
 
-def popAt_pushAt_eq (lctx : Nat → α) (x : α) :
-  (pos : Nat) → (n : Nat) → popLCtxAt (pushLCtxAt lctx x pos) pos n = lctx n
+def popAtRec_pushAtRec_eq (lctx : Nat → α) (x : α) :
+  (pos : Nat) → (n : Nat) → popLCtxAtRec (pushLCtxAtRec lctx x pos) pos n = lctx n
 | 0 => fun _ => rfl
 | pos' + 1 => fun n =>
   match n with
   | 0 => rfl
-  | n' + 1 => popAt_pushAt_eq (fun n => lctx (Nat.succ n)) x pos' n'
+  | n' + 1 => popAtRec_pushAtRec_eq (fun n => lctx (Nat.succ n)) x pos' n'
 
-def popAtDep_pushAtDep_eq
+def popAtDepRec_pushAtDepRec_eq
   {α : Sort w} {rty : Nat → α} {lctxty : α → Sort u}
   (lctx : ∀ n, lctxty (rty n)) {xty : α} (x : lctxty xty) : (pos n : Nat) →
-  HEq (@popLCtxAtDep _ (pushLCtxAt rty xty pos) lctxty
-        (@pushLCtxAtDep _ rty lctxty lctx xty x pos) pos n
+  HEq (@popLCtxAtDepRec _ (pushLCtxAtRec rty xty pos) lctxty
+        (@pushLCtxAtDepRec _ rty lctxty lctx xty x pos) pos n
       )
       (lctx n)
 | 0 => fun _ => HEq.rfl
 | pos' + 1 => fun n =>
   match n with
   | 0 => HEq.rfl
-  | n' + 1 => @popAtDep_pushAtDep_eq _ _ lctxty (fun n => lctx (Nat.succ n)) _ x pos' n'
+  | n' + 1 => @popAtDepRec_pushAtDepRec_eq _ _ lctxty (fun n => lctx (Nat.succ n)) _ x pos' n'
 
 end Auto.Embedding
