Auto/Embedding/LamBase.lean
@@ -915,67 +915,53 @@ end Example
 def LamTerm.bvarLiftIdx (idx : Nat) : LamTerm → LamTerm
 | .atom n     => .atom n
 | .base b     => .base b
-| .bvar n     => .bvar (popLCtxAt id idx n)
+| .bvar n     => .bvar (popLCtxAtRec id idx n)
 | .lam s t    => .lam s (t.bvarLiftIdx (Nat.succ idx))
 | .app fn arg => .app (fn.bvarLiftIdx idx) (arg.bvarLiftIdx idx)
 
 def LamTerm.bvarLift : LamTerm → LamTerm := LamTerm.bvarLiftIdx 0
 
-def LamTerm.bvarLifts (t : LamTerm) : (lvl : Nat) → LamTerm
+def LamTerm.bvarLiftsRec (t : LamTerm) : (lvl : Nat) → LamTerm
 | 0 => t
-| lvl' + 1 => (t.bvarLifts lvl').bvarLift
+| lvl' + 1 => (t.bvarLiftsRec lvl').bvarLift
 
-def LamTerm.bvarLifts_cast₁ {lvl : Nat} {rterm : LamTerm} (f : LamTerm → Sort u)
-  (H : f (LamTerm.bvarLifts (LamTerm.bvarLift rterm) lvl)) :
-  f (LamTerm.bvarLifts rterm (Nat.succ lvl)) :=
-  match lvl with
-  | 0 => H
-  | lvl' + 1 => LamTerm.bvarLifts_cast₁ (rterm:=rterm) (f := fun t => f (t.bvarLift)) H
-
-def LamTerm.bvarLifts_cast₂ {lvl : Nat} {rterm : LamTerm} (f : LamTerm → Sort u)
-  (H : f (LamTerm.bvarLifts rterm (Nat.succ lvl))) :
-  f (LamTerm.bvarLifts (LamTerm.bvarLift rterm) lvl) :=
-  match lvl with
-  | 0 => H
-  | _ + 1 => LamTerm.bvarLifts_cast₂ (rterm:=rterm) (f := fun t => f (t.bvarLift)) H
-
-private def LamWF.ofBVarLiftIdx_bvarAux
+private def LamWF.ofBVarLiftIdxRec_bvarAux
   (lctx : Nat → α) (pos n : Nat) :
-  pushLCtxAt lctx x pos (popLCtxAt id pos n) = lctx n := by
-  rw [popLCtxAt.comm id (pushLCtxAt lctx x pos)]; dsimp
-  rw [popAt_pushAt_eq]
+  pushLCtxAtRec lctx x pos (popLCtxAtRec id pos n) = lctx n := by
+  rw [popLCtxAtRec.comm id (pushLCtxAtRec lctx x pos)]; dsimp
+  rw [popAtRec_pushAtRec_eq]
 
-def LamWF.ofBVarLiftIdx {lamVarTy lctx} (idx : Nat) (rterm : LamTerm) :
+def LamWF.ofBVarLiftIdxRec {lamVarTy lctx} (idx : Nat) (rterm : LamTerm) :
   (HWF : LamWF lamVarTy ⟨lctx, rterm, rTy⟩) →
-  LamWF lamVarTy ⟨pushLCtxAt lctx x idx, rterm.bvarLiftIdx idx, rTy⟩
+  LamWF lamVarTy ⟨pushLCtxAtRec lctx x idx, rterm.bvarLiftIdx idx, rTy⟩
 | .ofAtom n => .ofAtom n
 | .ofBase b => .ofBase b
 | .ofBVar n => 
-  let IH := @LamWF.ofBVar lamVarTy (pushLCtxAt lctx x idx) (popLCtxAt id idx n)
-  LamWF.ofBVarLiftIdx_bvarAux lctx idx _ ▸ IH
+  let IH := @LamWF.ofBVar lamVarTy (pushLCtxAtRec lctx x idx) (popLCtxAtRec id idx n)
+  LamWF.ofBVarLiftIdxRec_bvarAux lctx idx _ ▸ IH
 | .ofLam (argTy:=argTy) (body:=body) bodyTy wfBody =>
   .ofLam (argTy:=argTy) bodyTy
     (body:=body.bvarLiftIdx (Nat.succ idx))
-    (LamWF.ofBVarLiftIdx (lctx:=pushLCtx lctx argTy) (Nat.succ idx) _ wfBody)
+    (LamWF.ofBVarLiftIdxRec (lctx:=pushLCtx lctx argTy) (Nat.succ idx) _ wfBody)
 | .ofApp argTy' HFn HArg =>
-  let IHFn := LamWF.ofBVarLiftIdx idx _ HFn
-  let IHArg := LamWF.ofBVarLiftIdx idx _ HArg
+  let IHFn := LamWF.ofBVarLiftIdxRec idx _ HFn
+  let IHArg := LamWF.ofBVarLiftIdxRec idx _ HArg
   .ofApp argTy' IHFn IHArg
 
-def LamWF.ofBVarLift {lamVarTy lctx} (rterm : LamTerm) 
+def LamWF.ofBVarLiftRec {lamVarTy lctx} (rterm : LamTerm) 
   (HWF : LamWF lamVarTy ⟨lctx, rterm, rTy⟩) :
   LamWF lamVarTy ⟨pushLCtx lctx x, rterm.bvarLift, rTy⟩ :=
-  LamWF.ofBVarLiftIdx 0 rterm HWF
+  LamWF.ofBVarLiftIdxRec 0 rterm HWF
 
 private def LamWF.bvarLiftIdx_correct_bvarAux {rty : Nat → α}
   {lctxty : α → Sort u} (lctx : ∀ n, lctxty (rty n))
   {xty : α} (x : lctxty xty) (pos n : Nat) :
-  HEq (pushLCtxAtDep lctx x pos (popLCtxAt id pos n)) (lctx n) := by
-  rw [popLCtxAt.commDep id (pushLCtxAtDep lctx x pos)]; simp
+  HEq (pushLCtxAtDepRec lctx x pos (popLCtxAtRec id pos n)) (lctx n) := by
+  rw [popLCtxAtRec.commDep id (pushLCtxAtDepRec lctx x pos)]; simp
   apply HEq.trans
-    (b := @popLCtxAtDep _ (pushLCtxAt rty xty pos) lctxty (fun n => pushLCtxAtDep lctx x pos n) pos n)
-  case h₁ => apply HEq.symm; apply @popLCtxAtDep.absorbAux'
-  case h₂ => apply popAtDep_pushAtDep_eq
+    (b := @popLCtxAtDepRec _ (pushLCtxAtRec rty xty pos) lctxty (fun n => pushLCtxAtDepRec lctx x pos n) pos n)
+  case h₁ => apply HEq.symm; apply @popLCtxAtDepRec.absorbAux'
+  case h₂ => apply popAtDepRec_pushAtDepRec_eq
 
 def LamWF.bvarLiftIdx_correct.{u}
   (lval : LamValuation.{u}) (lctxTy : Nat → LamSort) (idx : Nat)
@@ -983,27 +969,27 @@ def LamWF.bvarLiftIdx_correct.{u}
   {xty : LamSort} (x : LamSort.interp lval.ilVal.tyVal xty) :
   (rterm : LamTerm) → (HWF : LamWF lval.ilVal.toLamTyVal ⟨lctxTy, rterm, rTy⟩) →
   LamTerm.interp lval lctxTy lctxTerm HWF = LamTerm.interp lval
-    (pushLCtxAt lctxTy xty idx) (pushLCtxAtDep lctxTerm x idx)
-    (ofBVarLiftIdx idx rterm HWF)
+    (pushLCtxAtRec lctxTy xty idx) (pushLCtxAtDepRec lctxTerm x idx)
+    (ofBVarLiftIdxRec idx rterm HWF)
 | .atom n, .ofAtom _ => rfl
 | .base _, .ofBase _ => rfl
 | .bvar n, .ofBVar _ => by
-  simp [LamTerm.interp, ofBVarLiftIdx];
+  dsimp [LamTerm.interp, ofBVarLiftIdxRec];
   apply eq_of_heq
   apply HEq.trans (b:=LamTerm.interp lval
-    (pushLCtxAt lctxTy xty idx) (pushLCtxAtDep lctxTerm x idx)
-    (ofBVar (popLCtxAt id idx n)))
+    (pushLCtxAtRec lctxTy xty idx) (pushLCtxAtDepRec lctxTerm x idx)
+    (ofBVar (popLCtxAtRec id idx n)))
   case h.h₁ =>
-    simp [LamTerm.interp]
+    dsimp [LamTerm.interp]
     apply HEq.symm; apply LamWF.bvarLiftIdx_correct_bvarAux
   case h.h₂ =>
     congr
-    case e_2 => apply LamWF.ofBVarLiftIdx_bvarAux
+    case e_2 => apply LamWF.ofBVarLiftIdxRec_bvarAux
     case e_6 =>
       apply HEq.symm;
-      let h := @Auto.Embedding.Lam.LamWF.ofBVarLiftIdx_bvarAux LamSort xty lctxTy idx n
-      let φ := fun x => LamWF lval.ilVal.toLamTyVal ⟨pushLCtxAt lctxTy xty idx, LamTerm.bvarLiftIdx idx (LamTerm.bvar n), x⟩
-      exact (eqRec_heq (φ:=φ) h (ofBVar (popLCtxAt id idx n)))
+      let h := @Auto.Embedding.Lam.LamWF.ofBVarLiftIdxRec_bvarAux LamSort xty lctxTy idx n
+      let φ := fun x => LamWF lval.ilVal.toLamTyVal ⟨pushLCtxAtRec lctxTy xty idx, LamTerm.bvarLiftIdx idx (LamTerm.bvar n), x⟩
+      exact (eqRec_heq (φ:=φ) h (ofBVar (popLCtxAtRec id idx n)))
 | .lam argTy body, .ofLam bodyTy wfBody => funext (fun x' => LamWF.bvarLiftIdx_correct
     lval (pushLCtx lctxTy argTy) (Nat.succ idx)
     (pushLCtxDep lctxTerm x') x body wfBody)
@@ -1020,7 +1006,7 @@ def LamWF.bvarLift_correct.{u}
   (rterm : LamTerm) → (HWF : LamWF lval.ilVal.toLamTyVal ⟨lctxTy, rterm, rTy⟩) →
   LamTerm.interp lval lctxTy lctxTerm HWF = LamTerm.interp lval
     (pushLCtx lctxTy xty) (pushLCtxDep lctxTerm x)
-    (ofBVarLift rterm HWF) :=
+    (ofBVarLiftRec rterm HWF) :=
   LamWF.bvarLiftIdx_correct lval lctxTy 0 lctxTerm x  
 
 -- Suppose we have `(λ x. func[body]) arg`
@@ -1030,36 +1016,36 @@ def LamWF.bvarLift_correct.{u}
 --   easy to see that the `lctx` which `arg` resides in is `popLCtxs lctx (idx + 1)`
 --   and the type of `arg` is `lctx idx`
 def LamWF.subst (ltv : LamTyVal) (idx : Nat)
-  (arg : LamTerm) (argTy : LamSort)
-  (body : LamTerm) (bodyTy : LamSort) :
+  {arg : LamTerm} {argTy : LamSort}
+  {body : LamTerm} {bodyTy : LamSort} :
   (lctx : Nat → LamSort) → 
-  (wfArg : LamWF ltv ⟨lctx, LamTerm.bvarLifts arg idx, argTy⟩) →
-  (wfBody : LamWF ltv ⟨pushLCtxAt lctx argTy idx, body, bodyTy⟩) →
+  (wfArg : LamWF ltv ⟨lctx, LamTerm.bvarLiftsRec arg idx, argTy⟩) →
+  (wfBody : LamWF ltv ⟨pushLCtxAtRec lctx argTy idx, body, bodyTy⟩) →
   (substed : LamTerm) × LamWF ltv ⟨lctx, substed, bodyTy⟩
 | lctx, _,     .ofAtom n => ⟨.atom n, .ofAtom _⟩
 | lctx, _,     .ofBase (b:=b) H => ⟨.base b, .ofBase H⟩
 | lctx, wfArg, .ofBVar n =>
   let lctxty := fun rty => (substed : LamTerm) × LamWF ltv { lctx := lctx, rterm := substed, rty := rty}
-  let arg' := LamTerm.bvarLifts arg idx
-  pushLCtxAtDep (rty:=lctx) (lctxty:=lctxty) (lctx := fun n => ⟨.bvar n, .ofBVar n⟩) (xty:=argTy) (x := ⟨arg', wfArg⟩) idx n
+  let arg' := LamTerm.bvarLiftsRec arg idx
+  pushLCtxAtDepRec (rty:=lctx) (lctxty:=lctxty) (lctx := fun n => ⟨.bvar n, .ofBVar n⟩) (xty:=argTy) (x := ⟨arg', wfArg⟩) idx n
 | lctx, wfArg, .ofLam (argTy:=argTy') bodyTy' (body:=body') H =>
-  let wfArg' := LamWF.ofBVarLift (lctx:=lctx) _ wfArg
-  let IHArg := LamWF.subst ltv (Nat.succ idx) _ _ _ _ _ wfArg' H
+  let wfArg' := LamWF.ofBVarLiftRec (lctx:=lctx) _ wfArg
+  let IHArg := LamWF.subst ltv (Nat.succ idx) _ wfArg' H
   ⟨.lam argTy' IHArg.fst, .ofLam _ IHArg.snd⟩
 | lctx, wfArg, .ofApp argTy' HFn HArg =>
-  let IHFn := LamWF.subst ltv idx _ _ _ _ _ wfArg HFn
-  let IHArg := LamWF.subst ltv idx _ _ _ _ _ wfArg HArg
+  let IHFn := LamWF.subst ltv idx _ wfArg HFn
+  let IHArg := LamWF.subst ltv idx _ wfArg HArg
   ⟨.app IHFn.fst IHArg.fst, .ofApp argTy' IHFn.snd IHArg.snd⟩
 
 def LamWF.subst_correct.{u}
   (lval : LamValuation.{u}) (idx : Nat)
   {arg : LamTerm} {argTy : LamSort} {body : LamTerm} {bodyTy : LamSort} :
   (lctxTy : Nat → LamSort) → (lctxTerm : ∀ n, (lctxTy n).interp lval.ilVal.tyVal) →
-  (wfArg : LamWF lval.ilVal.toLamTyVal ⟨lctxTy, LamTerm.bvarLifts arg idx, argTy⟩) →
-  (wfBody : LamWF lval.ilVal.toLamTyVal ⟨pushLCtxAt lctxTy argTy idx, body, bodyTy⟩) →
-  let wfSubst := LamWF.subst lval.ilVal.toLamTyVal idx arg argTy body bodyTy lctxTy wfArg wfBody
-  (LamTerm.interp lval (pushLCtxAt lctxTy argTy idx)
-    (pushLCtxAtDep lctxTerm (LamTerm.interp lval lctxTy lctxTerm wfArg) idx) wfBody
+  (wfArg : LamWF lval.ilVal.toLamTyVal ⟨lctxTy, LamTerm.bvarLiftsRec arg idx, argTy⟩) →
+  (wfBody : LamWF lval.ilVal.toLamTyVal ⟨pushLCtxAtRec lctxTy argTy idx, body, bodyTy⟩) →
+  let wfSubst := LamWF.subst lval.ilVal.toLamTyVal idx lctxTy wfArg wfBody
+  (LamTerm.interp lval (pushLCtxAtRec lctxTy argTy idx)
+    (pushLCtxAtDepRec lctxTerm (LamTerm.interp lval lctxTy lctxTerm wfArg) idx) wfBody
   = LamTerm.interp lval lctxTy lctxTerm wfSubst.snd)
 | lctxTy, lctxTerm, wfArg, .ofAtom n => rfl
 | lctxTy, lctxTerm, wfArg, .ofBase b => rfl
@@ -1069,10 +1055,10 @@ def LamWF.subst_correct.{u}
   let f := fun (rty : LamSort) (r : lctxty rty) => LamTerm.interp lval lctxTy lctxTerm r.snd
   let lctx := fun n => (⟨LamTerm.bvar n, .ofBVar n⟩ : @Sigma LamTerm
     (fun substed => LamWF lval.ilVal.toLamTyVal ⟨lctxTy, substed, lctxTy n⟩))
-  Eq.symm (pushLCtxAtDep.comm (β:=β) (lctxty:=lctxty) f lctx ⟨_, wfArg⟩ _ _)
+  Eq.symm (pushLCtxAtDepRec.comm (β:=β) (lctxty:=lctxty) f lctx ⟨_, wfArg⟩ _ _)
 | lctxTy, lctxTerm, wfArg, .ofLam (argTy:=argTy') bodyTy' (body:=body') H =>
   funext (fun x =>
-    let wfArg' := LamWF.ofBVarLift (lctx:=lctxTy) _ wfArg
+    let wfArg' := LamWF.ofBVarLiftRec (lctx:=lctxTy) _ wfArg
     let IH := LamWF.subst_correct lval (.succ idx) (pushLCtx lctxTy argTy') (pushLCtxDep lctxTerm x) wfArg' H
     Eq.trans (by
       dsimp [LamTerm.interp]
