Auto/Embedding/LamThm.lean
@@ -1,0 +1,35 @@
+import Auto.Embedding.LamBase
+
+namespace Auto.Embedding.Lam
+
+def LamTerm.bvarLifts (t : LamTerm) (lvl : Nat) : LamTerm :=
+  match t with
+  | .atom n     => .atom n
+  | .base b     => .base b
+  | .bvar n     => .bvar (Nat.add n lvl)
+  | .lam s t    => .lam s (t.bvarLifts lvl)
+  | .app fn arg => .app (fn.bvarLifts lvl) (arg.bvarLifts lvl)
+
+def LamTerm.subst (idx : Nat) (arg : LamTerm) : (body : LamTerm) → LamTerm
+| .atom n     => .atom n
+| .base b     => .base b
+| .bvar n     => pushLCtxAt LamTerm.bvar (arg.bvarLifts idx) idx n
+| .lam s body => .lam s (LamTerm.subst (.succ idx) arg body)
+| .app fn arg' => .app (LamTerm.subst idx arg fn) (LamTerm.subst idx arg arg')
+
+def LamTerm.subst_correct (ltv : LamTyVal) (idx : Nat)
+  {arg : LamTerm} {argTy : LamSort}
+  {body : LamTerm} {bodyTy : LamSort}
+  (lctx : Nat → LamSort) :
+  (wfArg : LamWF ltv ⟨lctx, LamTerm.bvarLiftsRec arg idx, argTy⟩) →
+  (wfBody : LamWF ltv ⟨pushLCtxAtRec lctx argTy idx, body, bodyTy⟩) →
+  LamTerm.subst idx arg body = (LamWF.subst ltv idx lctx wfArg wfBody).fst
+| wfArg, .ofAtom n => rfl
+| wfArg, .ofBase (b:=b) H => rfl
+| wfArg, .ofBVar n => by
+  simp [LamTerm.subst, LamWF.subst]
+  sorry
+| wfArg, .ofLam (argTy:=argTy') bodyTy' (body:=body') H => sorry
+| wfArg, .ofApp argTy' HFn HArg => sorry
+
+end Auto.Embedding.Lam
